dist/gcc-compatible/Hacl_Bignum4096.c
@@ -695,10 +695,10 @@ exp_vartime_precomp(
   uint64_t *ctx_r20 = ctx + (uint32_t)64U;
   from(ctx_n0, mu, ctx_r20, t0);
   memcpy(t1, aM, (uint32_t)64U * sizeof (uint64_t));
-  for (uint32_t i = (uint32_t)0U; i < (uint32_t)15U; i++)
+  for (uint32_t i = (uint32_t)0U; i < (uint32_t)14U; i++)
   {
-    uint64_t *t11 = table + i * (uint32_t)64U;
-    uint64_t *t2 = table + i * (uint32_t)64U + (uint32_t)64U;
+    uint64_t *t11 = table + (i + (uint32_t)1U) * (uint32_t)64U;
+    uint64_t *t2 = table + (i + (uint32_t)2U) * (uint32_t)64U;
     uint64_t *ctx_n = ctx;
     amont_mul(ctx_n, mu, aM, t11, t2);
   }
@@ -842,10 +842,10 @@ exp_consttime_precomp(
   uint64_t *ctx_r20 = ctx + (uint32_t)64U;
   from(ctx_n0, mu, ctx_r20, t0);
   memcpy(t1, aM, (uint32_t)64U * sizeof (uint64_t));
-  for (uint32_t i = (uint32_t)0U; i < (uint32_t)15U; i++)
+  for (uint32_t i = (uint32_t)0U; i < (uint32_t)14U; i++)
   {
-    uint64_t *t11 = table + i * (uint32_t)64U;
-    uint64_t *t2 = table + i * (uint32_t)64U + (uint32_t)64U;
+    uint64_t *t11 = table + (i + (uint32_t)1U) * (uint32_t)64U;
+    uint64_t *t2 = table + (i + (uint32_t)2U) * (uint32_t)64U;
     uint64_t *ctx_n = ctx;
     amont_mul(ctx_n, mu, aM, t11, t2);
   }
