dist/gcc-compatible/Hacl_Ed25519.c
@@ -1331,10 +1331,10 @@ void Hacl_Impl_Ed25519_Ladder_point_mul(uint64_t *result, uint8_t *scalar, uint6
   uint64_t *t1 = table + (uint32_t)20U;
   Hacl_Impl_Ed25519_Ladder_make_point_inf(t0);
   memcpy(t1, q, (uint32_t)20U * sizeof (uint64_t));
-  for (uint32_t i = (uint32_t)0U; i < (uint32_t)15U; i++)
+  for (uint32_t i = (uint32_t)0U; i < (uint32_t)14U; i++)
   {
-    uint64_t *t11 = table + i * (uint32_t)20U;
-    uint64_t *t2 = table + i * (uint32_t)20U + (uint32_t)20U;
+    uint64_t *t11 = table + (i + (uint32_t)1U) * (uint32_t)20U;
+    uint64_t *t2 = table + (i + (uint32_t)2U) * (uint32_t)20U;
     Hacl_Impl_Ed25519_PointAdd_point_add(t2, q, t11);
   }
   Hacl_Impl_Ed25519_Ladder_make_point_inf(result);
@@ -1440,10 +1440,10 @@ point_mul_double_vartime(
   uint64_t *t10 = table1 + (uint32_t)20U;
   Hacl_Impl_Ed25519_Ladder_make_point_inf(t00);
   memcpy(t10, q1, (uint32_t)20U * sizeof (uint64_t));
-  for (uint32_t i = (uint32_t)0U; i < (uint32_t)15U; i++)
+  for (uint32_t i = (uint32_t)0U; i < (uint32_t)14U; i++)
   {
-    uint64_t *t11 = table1 + i * (uint32_t)20U;
-    uint64_t *t2 = table1 + i * (uint32_t)20U + (uint32_t)20U;
+    uint64_t *t11 = table1 + (i + (uint32_t)1U) * (uint32_t)20U;
+    uint64_t *t2 = table1 + (i + (uint32_t)2U) * (uint32_t)20U;
     Hacl_Impl_Ed25519_PointAdd_point_add(t2, q1, t11);
   }
   uint64_t table2[320U] = { 0U };
@@ -1451,10 +1451,10 @@ point_mul_double_vartime(
   uint64_t *t1 = table2 + (uint32_t)20U;
   Hacl_Impl_Ed25519_Ladder_make_point_inf(t0);
   memcpy(t1, q2, (uint32_t)20U * sizeof (uint64_t));
-  for (uint32_t i = (uint32_t)0U; i < (uint32_t)15U; i++)
+  for (uint32_t i = (uint32_t)0U; i < (uint32_t)14U; i++)
   {
-    uint64_t *t11 = table2 + i * (uint32_t)20U;
-    uint64_t *t2 = table2 + i * (uint32_t)20U + (uint32_t)20U;
+    uint64_t *t11 = table2 + (i + (uint32_t)1U) * (uint32_t)20U;
+    uint64_t *t2 = table2 + (i + (uint32_t)2U) * (uint32_t)20U;
     Hacl_Impl_Ed25519_PointAdd_point_add(t2, q2, t11);
   }
   Hacl_Impl_Ed25519_Ladder_make_point_inf(result);
