dist/gcc-compatible/Hacl_GenericField64.c
@@ -342,10 +342,10 @@ Hacl_GenericField64_exp_consttime(
     uint64_t *ctx_r20 = ctx + len1;
     Hacl_Bignum_Montgomery_bn_from_mont_u64(len1, ctx_n0, k1.mu, ctx_r20, t0);
     memcpy(t1, aMc, len1 * sizeof (uint64_t));
-    for (uint32_t i = (uint32_t)0U; i < (uint32_t)15U; i++)
+    for (uint32_t i = (uint32_t)0U; i < (uint32_t)14U; i++)
     {
-      uint64_t *t11 = table + i * len1;
-      uint64_t *t2 = table + i * len1 + len1;
+      uint64_t *t11 = table + (i + (uint32_t)1U) * len1;
+      uint64_t *t2 = table + (i + (uint32_t)2U) * len1;
       uint64_t *ctx_n = ctx;
       Hacl_Bignum_Montgomery_bn_mont_mul_u64(len1, ctx_n, k1.mu, aMc, t11, t2);
     }
@@ -510,10 +510,10 @@ Hacl_GenericField64_exp_vartime(
     uint64_t *ctx_r20 = ctx + len1;
     Hacl_Bignum_Montgomery_bn_from_mont_u64(len1, ctx_n0, k1.mu, ctx_r20, t0);
     memcpy(t1, aMc, len1 * sizeof (uint64_t));
-    for (uint32_t i = (uint32_t)0U; i < (uint32_t)15U; i++)
+    for (uint32_t i = (uint32_t)0U; i < (uint32_t)14U; i++)
     {
-      uint64_t *t11 = table + i * len1;
-      uint64_t *t2 = table + i * len1 + len1;
+      uint64_t *t11 = table + (i + (uint32_t)1U) * len1;
+      uint64_t *t2 = table + (i + (uint32_t)2U) * len1;
       uint64_t *ctx_n = ctx;
       Hacl_Bignum_Montgomery_bn_mont_mul_u64(len1, ctx_n, k1.mu, aMc, t11, t2);
     }
